---
layout: post
title:  "Expectation Maximization from Jensen's inequality"
date:   2018-06-03 23:00:00 -0700
categories: ML
---

#### __Abstract__
In this post we introduce a common view on Expectation Maximization using Jensen's inequality.

#### __References__
[Andrew's note]: http://cs229.stanford.edu/notes/cs229-notes8.pdf
[wikipedia]: https://en.wikipedia.org/wiki/Jensen%27s_inequality

[Andrew's note]


### __EM and maximum likelihood estimation__
The goal of EM is to maximize the likelihood of observed variable X explained by hidden variable Z under a model with 
parameters $$\theta$$. Noted that when Z is known (usually as labels), this problem becomes a supervised learning problem and 
it can be solved directly using maximum likelihood estimaation instead of EM. For a training dataset with size $$n$$, the expected log likelihood of
a dataset with instances $$x_1$$, $$x_2$$, ... $$x_n$$ drawn from distribution $$p_{true}(x)$$ is given by:

$$
\begin{align}
    \mathbb{E}_x (\log p_{\theta}(x)) \approx \frac{1}{n} \sum_{i=1}^{n} \log p_{\theta}(x_i), \quad x_i \sim p_{true}(x) \tag{0}
\end{align}
$$

Our objective is to maximize (0) by adjusting $$\theta$$

$$
\begin{align}
    \operatorname*{argmax}_{\theta} \mathbb{E}_x (\log p_{\theta}(x_i)) &= \operatorname*{argmax}_{\theta} n \cdot \mathbb{E}_x (\log p_{\theta}(x_i)) \\
                                                                        &= \operatorname*{argmax}_{\theta} \sum_{i=1}^{n} \log p_{\theta}(x_i) \\
                                                                        &= \operatorname*{argmax}_{\theta} \sum_{i=1}^{n} \log \sum_{z_i} p_{\theta}(x_i , z_i) \\
                                                                        &= \operatorname*{argmax}_{\theta} l(\theta) \tag{1}
\end{align}
$$


### __Derivation from Jensen's inequality__
Starting from (1), derivation using Jensen's inequality adds a "helper" distribution $$q$$ such that

$$
\begin{align}
    l(\theta) &= \sum_{i=1}^{n} \log \sum_{z_i} p_{\theta}(x_i , z_i)  \\
              &= \sum_{i=1}^{n} \log \sum_{z_i} \frac{q(z_i) p_{\theta}(x_i , z_i)}{q(z_i)} \tag{2} \\
              & \geq \sum_{i=1}^{n} \sum_{z_i} q(z_i) \log \frac{p_{\theta}(x_i , z_i)}{q(z_i)} \tag{3}
\end{align}
$$

(2) is greater than or equal to (3) because Jensen's inequaitliy states that $$f(E[Y]) \geq E[f(Y)]$$ 
if $$f$$ is a concave function (for more details, look at [Andrew's note] or [wikipedia]). 
In our case, $$f$$ is $$log$$ which is a concave function and $$Y$$ is $$\frac{p(x_i , z_i; \theta)}{q(z_i)}$$. 
Using (3) as a lower bound of (2), 
we want to raise (3) as close as possible to (2) such that (3) $$=$$ (2) to maximize the likelihood. 
For this, Jensen's inequality also states that when $$Y$$ is constant, $$f(E[Y]) = E[f(Y)]$$. 
Therefore, we can construct $$q$$ such that Y is equal to some constant c as follow

$$
    Y = \frac{p_{\theta}(x_i , z_i)}{q(z_i)} = c \tag{4}
$$ 

If we assume each instance has the same corresponding constant c, then we have

$$
    \frac{\sum_{z_i} p_{\theta}(x_i , z_i)}{\sum_{z_i} q(z_i)} = c \tag{5}
$$

Given $$q(z_i)$$ is a probability distribution and $$\sum_{z_i} q(z_i) = 1$$, we have

$$
    c = \sum_{z_i} p_{\theta}(x_i , z_i) = p_{\theta}(x_i) \tag{6}
$$

Therefore, $$q(z_i)$$ can be written as follow

$$
    q(z_i) = \frac{p_{\theta}(x_i , z_i)}{p_{\theta}(x_i)} = p_{\theta}(z_i | x_i) \tag{7}
$$

### __Expectation Maximization__
(7) is our E step

$$
    q(z_i) = p_{\theta}(z_i | x_i) \tag{E-step}
$$

Using (7) to replace $$q(z_i)$$ in (3), we obtain our M step assuming $$p_{\theta}(x_i \vert z_i)$$ is constant

$$
\begin{align}
    \theta_{new} &= \operatorname*{argmax}_{\theta} \sum_{i=1}^{n} \sum_{z_i} p_{\theta}(z_i | x_i) \log \frac{p_{\theta}(x_i , z_i)}{p_{\theta}(z_i | x_i)} \\
                 &= \operatorname*{argmax}_{\theta} \sum_{i=1}^{n} \sum_{z_i} p_{\theta}(z_i | x_i) \log p_{\theta}(x_i , z_i) - \sum_{z_i} p_{\theta}(z_i | x_i) \log p_{\theta}(z_i | x_i) \\
                 &= \operatorname*{argmax}_{\theta} \sum_{i=1}^{n} \sum_{z_i} p_{\theta}(z_i | x_i) \log p_{\theta}(x_i , z_i) - C \\
                 &= \operatorname*{argmax}_{\theta} \sum_{i=1}^{n} \sum_{z_i} p_{\theta}(z_i | x_i) \log p_{\theta}(x_i , z_i) \tag{M-step}
\end{align}
$$

#### *__Notes__*
For (5), it seems this assumption is necessary but ignored from [Andrew's note] and some other sources. 
How does such assumption affect the construction of $$q(z_i)$$?




